@prefix : <http://www.semanticweb.org/tomas/ontologies/2023/10/untitled-ontology-3/> .
@prefix owl: <http://www.w3.org/2002/07/owl#> .
@prefix rdf: <http://www.w3.org/1999/02/22-rdf-syntax-ns#> .
@prefix xml: <http://www.w3.org/XML/1998/namespace> .
@prefix xsd: <http://www.w3.org/2001/XMLSchema#> .
@prefix rdfs: <http://www.w3.org/2000/01/rdf-schema#> .
@prefix fabio: <http://purl.org/spar/fabio/> .
@base <http://www.semanticweb.org/tomas/ontologies/2023/10/untitled-ontology-3/> .

<https://w3id.org/ocs/ont/papers/> rdf:type owl:Ontology ;
                                    rdfs:comment "This ontology describes properties used in OpenCS knowledge graph about research articles from the domain of Computer Science." .

#################################################################
#    Object Properties
#################################################################

###  http://www.semanticweb.org/tomas/ontologies/2023/10/untitled-ontology-3/hasRelatedPapers
:hasRelatedPapers rdf:type owl:ObjectProperty ,
                           owl:SymmetricProperty ,
                           owl:ReflexiveProperty ;
                  rdfs:domain fabio:ResearchPaper ;
                  rdfs:range fabio:ResearchPaper ;
                  rdfs:comment "Indicates that a research paper has similar content to another research paper, determined by the cosine similarity of their embeddings." .


###  http://www.semanticweb.org/tomas/ontologies/2023/10/untitled-ontology-3/hasRelatedTopics
:hasRelatedTopics rdf:type owl:ObjectProperty ,
                           owl:IrreflexiveProperty ;
                  rdfs:domain fabio:ResearchPaper ;
                  rdfs:comment "Specifies a list of topics or concepts that are related to the given research paper." .


#################################################################
#    Data properties
#################################################################

###  http://www.semanticweb.org/tomas/ontologies/2023/10/untitled-ontology-3/hasWordEmbedding
:hasWordEmbedding rdf:type owl:DatatypeProperty ,
                           owl:FunctionalProperty ;
                  rdfs:domain fabio:ResearchPaper ;
                  rdfs:range xsd:string ;
                  rdfs:comment "Represents the embedded vector of the title and abstract of a given research paper." .


###  http://www.semanticweb.org/tomas/ontologies/2023/10/untitled-ontology-3/relationScore
:relationScore rdf:type owl:DatatypeProperty ,
                        owl:FunctionalProperty ;
               rdfs:range xsd:float ;
               rdfs:comment "Quantifies the degree of relationship between a given research paper and a topic. The higher the value, the stronger the association, with no fixed range specified." .


###  http://www.semanticweb.org/tomas/ontologies/2023/10/untitled-ontology-3/similarityScore
:similarityScore rdf:type owl:DatatypeProperty ,
                          owl:FunctionalProperty ;
                 rdfs:domain fabio:ResearchPaper ;
                 rdfs:range xsd:float ;
                 rdfs:comment "Specifies the cosine similarity between the embeddings of two research papers, indicating the degree of similarity in their content." .


#################################################################
#    Classes
#################################################################

###  http://purl.org/spar/fabio/ResearchPaper
fabio:ResearchPaper rdf:type owl:Class .


###  Generated by the OWL API (version 4.5.26.2023-07-17T20:34:13Z) https://github.com/owlcs/owlapi
