@prefix : <https://w3id.org/ocs/ont/papers#> .
@prefix owl: <http://www.w3.org/2002/07/owl#> .
@prefix rdf: <http://www.w3.org/1999/02/22-rdf-syntax-ns#> .
@prefix xml: <http://www.w3.org/XML/1998/namespace> .
@prefix xsd: <http://www.w3.org/2001/XMLSchema#> .
@prefix rdfs: <http://www.w3.org/2000/01/rdf-schema#> .
@prefix skos: <http://www.w3.org/2004/02/skos/core#> .
@prefix fabio: <http://purl.org/spar/fabio/> .
@prefix ocs_papers: <https://w3id.org/ocs/ont/papers/> .
@base <https://w3id.org/ocs/ont/papers> .

<https://w3id.org/ocs/ont/papers> rdf:type owl:Ontology ;
                                   rdfs:comment "This ontology describes properties used in OpenCS knowledge graph about research articles from the domain of Computer Science."@en ;
                                   rdfs:label "OpenCS Knowledge Graph ontology"@en .

#################################################################
#    Object Properties
#################################################################

###  https://w3id.org/ocs/ont/papers/hasRelated
ocs_papers:hasRelated rdf:type owl:ObjectProperty ,
                               owl:InverseFunctionalProperty ,
                               owl:IrreflexiveProperty ;
                      rdfs:domain fabio:ResearchPaper ;
                      rdfs:range ocs_papers:RelatedObjectRelation ;
                      rdfs:comment "Represents a relation between research paper and other object. Points to RelatedObjectRelation class. Other properties are then used to further describe the relation."@en .


###  https://w3id.org/ocs/ont/papers/hasRelatedPaper
ocs_papers:hasRelatedPaper rdf:type owl:ObjectProperty ;
                           rdfs:subPropertyOf ocs_papers:hasRelated ;
                           rdf:type owl:InverseFunctionalProperty ,
                                    owl:IrreflexiveProperty ;
                           rdfs:domain fabio:ResearchPaper ;
                           rdfs:range ocs_papers:RelatedPaperRelation ;
                           rdfs:comment "Indicates that a research paper has similar content to another research paper, determined by the cosine similarity of their embeddings."@en .


###  https://w3id.org/ocs/ont/papers/hasRelatedTopic
ocs_papers:hasRelatedTopic rdf:type owl:ObjectProperty ;
                           rdfs:subPropertyOf ocs_papers:hasRelated ;
                           rdf:type owl:InverseFunctionalProperty ,
                                    owl:IrreflexiveProperty ;
                           rdfs:domain fabio:ResearchPaper ;
                           rdfs:range ocs_papers:RelatedTopicRelation ;
                           rdfs:comment "Specifies a list of topics or concepts that are related to the given research paper."@en .


###  https://w3id.org/ocs/ont/papers/hasRelationTarget
ocs_papers:hasRelationTarget rdf:type owl:ObjectProperty ,
                                      owl:FunctionalProperty ,
                                      owl:IrreflexiveProperty ;
                             rdfs:domain ocs_papers:RelatedObjectRelation ;
                             rdfs:comment "Target of the relation. An object that is associated with a given research paper."@en .


#################################################################
#    Data properties
#################################################################

###  https://w3id.org/ocs/ont/papers/hasRelationScore
ocs_papers:hasRelationScore rdf:type owl:DatatypeProperty ,
                                     owl:FunctionalProperty ;
                            rdfs:domain ocs_papers:RelatedObjectRelation ;
                            rdfs:range xsd:float ;
                            rdfs:comment "Quantifies how much the target of the relationship is related to a given research paper."@en .


###  https://w3id.org/ocs/ont/papers/hasWordEmbedding
ocs_papers:hasWordEmbedding rdf:type owl:DatatypeProperty ,
                                     owl:FunctionalProperty ;
                            rdfs:domain fabio:ResearchPaper ;
                            rdfs:range xsd:string ;
                            rdfs:comment "Represents the embedded vector of the title and abstract of a given research paper."@en .


#################################################################
#    Classes
#################################################################

###  http://purl.org/spar/fabio/ResearchPaper
fabio:ResearchPaper rdf:type owl:Class .


###  http://www.w3.org/2004/02/skos/core#Concept
skos:Concept rdf:type owl:Class .


###  https://w3id.org/ocs/ont/papers/RelatedObjectRelation
ocs_papers:RelatedObjectRelation rdf:type owl:Class ;
                                 rdfs:comment "A helper class used to better desribe relation between a given research paper and other object e.g. another paper or a concept."@en .


###  https://w3id.org/ocs/ont/papers/RelatedPaperRelation
ocs_papers:RelatedPaperRelation rdf:type owl:Class ;
                                rdfs:subClassOf ocs_papers:RelatedObjectRelation ,
                                                [ rdf:type owl:Restriction ;
                                                  owl:onProperty ocs_papers:hasRelationTarget ;
                                                  owl:allValuesFrom fabio:ResearchPaper
                                                ] ;
                                rdfs:comment "A helper class to better decribe relationship between two research papers."@en .


###  https://w3id.org/ocs/ont/papers/RelatedTopicRelation
ocs_papers:RelatedTopicRelation rdf:type owl:Class ;
                                rdfs:subClassOf ocs_papers:RelatedObjectRelation ,
                                                [ rdf:type owl:Restriction ;
                                                  owl:onProperty ocs_papers:hasRelationTarget ;
                                                  owl:allValuesFrom skos:Concept
                                                ] ;
                                rdfs:comment "A helper class to better describe relation between a given research paper and a relevant concept."@en .


###  Generated by the OWL API (version 4.5.9.2019-02-01T07:24:44Z) https://github.com/owlcs/owlapi
